max max max max max

Iterator/Combinators/FlatMap.lean
@@ -67,96 +67,93 @@ section FlatMap
 
 section FlattenDef
 
-universe u v
+variable {α : Type w} {α' : Type u} {β : Type v} {β' : Type w} {α₂ : Type w} {α₂' : Type u₂}
+    {γ : Type x} {γ' : Type w} {m : Type w → Type w'} {f : β → α₂}
 
-variable {α : Type u} {α' : Type u'}  {β : Type v}
-  {m : Type w → Type w'}
-  [Iterator α m α'] [Iterator α' m β]
-
-structure Flatten (α : Type u) (α' : Type u') where
+structure FlatMap (α : Type w) (f : β → α₂) where
   it₁ : α
-  it₂ : Option α'
+  it₂ : Option α₂
 
-@[inline]
-def Flatten.init (it : α) (α' : Type u'): Flatten α α' :=
+@[always_inline, inline]
+def FlatMap.init (it : α) (f : β → α₂) : FlatMap α f :=
   ⟨it, none⟩
 
-@[inline]
-def flattenStepNone (m : Type w → Type w') [Monad m] [Iterator α m α'] [Iterator α' m β] (it₁ : α) :
-    Iteration m (RawStep (Flatten α α') β) :=
+variable (m) in
+@[always_inline, inline]
+def flatMapStepNone (it₁ : α) [Monad m] [Iterator α α' m β] [Iterator α₂ α₂' m γ] :
+    IterationT m (RawStep (FlatMap α f) (Iterator.βInternal (α := α₂) (m := m))) :=
   matchStep it₁
-    (fun it₁' b => pure <| .skip { it₁ := it₁', it₂ := some b } ⟨⟩)
+    (fun it₁' b => pure <| .skip ⟨it₁', some (f b)⟩ ⟨⟩)
     (fun it₁' => pure <| .skip { it₁ := it₁', it₂ := none } ⟨⟩)
     (pure <| .done ⟨⟩)
 
-variable (f) in
-@[inline]
-def flattenStepSome (m : Type w → Type w') [Monad m] [Iterator α m α'] [Iterator α' m β] (it₁ : α) (it₂ : α') :
-    Iteration m (RawStep (Flatten α α') β) :=
+variable (m) in
+@[always_inline, inline]
+def flatMapStepSome [Monad m] [Iterator α α' m β] [Iterator α₂ α₂' m γ] (it₁ : α) (it₂ : α₂) :
+    IterationT m (RawStep (FlatMap α f) (Iterator.βInternal (α := α₂) (m := m))) :=
   matchStep it₂
-    (fun it₂' b => pure <| .yield { it₁ := it₁, it₂ := some it₂' } b ⟨⟩)
+    (fun it₂' b => pure <| .yield { it₁ := it₁, it₂ := some it₂' } (Iterator.βEquiv.hom b) ⟨⟩)
     (fun it₂' => pure <| .skip { it₁ := it₁, it₂ := some it₂' } ⟨⟩)
-    (flattenStepNone m it₁)
+    (flatMapStepNone m it₁)
 
-instance [Monad m] [Iterator α m α'] [Iterator α' m β] : Iterator (Flatten α α') m β :=
-  Iteration.instIterator fun
-    | { it₁, it₂ := none } => flattenStepNone m it₁
-    | { it₁, it₂ := some it₂ } => flattenStepSome m it₁ it₂
-
-@[inline]
-def Iter.flatten [Monad m] [i₁ : Iterator α m α'] [i₂ : Iterator α' m β] (it : Iter (α := α) m α') :=
-  toIter m <| Flatten.init it.inner α'
+instance [Monad m] [Iterator α α' m β] [Iterator α₂ α₂' m γ] : SimpleIterator (FlatMap α f) (α' × Option α₂') m γ where
+  βInternal := Iterator.βInternal (α := α₂) (m := m)
+  αEquiv := sorry
+  βEquiv := Iterator.βEquiv
+  step it := match it with
+    | { it₁, it₂ := none } => flatMapStepNone m it₁
+    | { it₁, it₂ := some it₂ } => flatMapStepSome m it₁ it₂
 
 end FlattenDef
 
 section Finite
 
-universe u v
+variable {α : Type w} {α' : Type u} {β : Type v} {β' : Type w} {α₂ : Type w} {α₂' : Type u₂}
+    {γ : Type x} {γ' : Type w} {m : Type w → Type w'} {f : β → α₂}
 
-variable {α : Type u} {α' : Type u'} {β : Type v} {m : Type w → Type w'}
-
-def Flatten.lex (r₁ : α → α → Prop) (r₂ : α' → α' → Prop) : Flatten α α' → Flatten α α' → Prop :=
+def FlatMap.lex (r₁ : α → α → Prop) (r₂ : α₂ → α₂ → Prop) : FlatMap α f → FlatMap α f → Prop :=
   InvImage (Prod.Lex r₁ (Option.lt r₂)) (fun it => (it.it₁, it.it₂))
 
-theorem Flatten.lex_of_left {r₁ : α → α → Prop} {r₂ : α' → α' → Prop} {it it'}
-    (h : r₁ it'.it₁ it.it₁) : Flatten.lex r₁ r₂ it' it :=
+theorem FlatMap.lex_of_left {r₁ : α → α → Prop} {r₂ : α₂ → α₂ → Prop} {it it'}
+    (h : r₁ it'.it₁ it.it₁) : FlatMap.lex (f := f) r₁ r₂ it' it :=
   Prod.Lex.left _ _ h
 
-theorem Flatten.lex_of_right {r₁ : α → α → Prop} {r₂ : α' → α' → Prop} {it₁ it₂ it₂'}
-    (h : r₂ it₂' it₂) : Flatten.lex r₁ r₂ ⟨it₁, it₂'⟩ ⟨it₁, it₂⟩ :=
+theorem FlatMap.lex_of_right {r₁ : α → α → Prop} {r₂ : α₂ → α₂ → Prop} {it₁ it₂ it₂'}
+    (h : r₂ it₂' it₂) : FlatMap.lex (f := f) r₁ r₂ ⟨it₁, it₂'⟩ ⟨it₁, it₂⟩ :=
   Prod.Lex.right _ h
 
-def rel (m : Type w → Type w') [Iterator α m α'] [Iterator α' m β] : Flatten α α' → Flatten α α' → Prop :=
-  Flatten.lex
+variable (m f) in
+def rel [Iterator α α' m β] [Iterator α₂ α₂' m γ] : FlatMap α f → FlatMap α f → Prop :=
+  FlatMap.lex
     (InvImage FiniteIteratorWF.lt (finiteIteratorWF (m := m)))
     (InvImage FiniteIteratorWF.lt (finiteIteratorWF (m := m)))
 
 theorem descending_flattenStepNone
-    [Monad m] [Iterator α m α'] [Iterator α' m β] {it₁ : α} {it' : Flatten α α'}
-    (h : ((ULift.up.{v} ∘ IterStep.successor) <$> flattenStepNone m it₁).prop (ULift.up <| some it')) :
+    [Monad m] [Iterator α α' m β] [Iterator α₂ α₂' m γ] {it₁ : α} {it' : FlatMap α f}
+    (h : (IterStep.successor <$> flatMapStepNone m it₁).property (some it')) :
     (finiteIteratorWF (m := m) it'.it₁).lt (finiteIteratorWF it₁) := by
-  simp only [flattenStepNone] at h
-  have := prop_successor_matchStep h
+  simp only [flatMapStepNone] at h
+  have := successor_matchStep h
   obtain ⟨it'', b, hy, h⟩ | ⟨it'', hs, h⟩ | ⟨hd, h⟩ := this
-  · cases up_successor_skip.mp h
+  · cases successor_skip.mp h
     exact Or.inl ⟨_, hy⟩
-  · cases up_successor_skip.mp h
+  · cases successor_skip.mp h
     exact Or.inr hs
-  · cases up_successor_done.mp h
+  · cases successor_done.mp h
 
 theorem descending_flattenStepSome
-    [Monad m] [Iterator α m α'] [Iterator α' m β] {it₁ : α} {it₂ : α'} {it' : Flatten α α'}
-    (h : ((ULift.up.{v} ∘ IterStep.successor) <$> flattenStepSome m it₁ it₂).prop (ULift.up <| some it')) :
-    rel m it' { it₁ := it₁, it₂ := some it₂ } := by
-  simp only [flattenStepSome] at h
-  obtain ⟨it', b, hy, h⟩ | ⟨it', hs, h⟩ | ⟨hd, h⟩ := prop_successor_matchStep h
-  · cases up_successor_yield.mp h
-    apply Flatten.lex_of_right
+    [Monad m] [Iterator α α' m β] [Iterator α₂ α₂' m γ] {it₁ : α} {it₂ : α₂} {it' : FlatMap α f}
+    (h : (IterStep.successor <$> flatMapStepSome m it₁ it₂).property (some it')) :
+    rel m f it' { it₁ := it₁, it₂ := some it₂ } := by
+  simp only [flatMapStepSome] at h
+  obtain ⟨it', b, hy, h⟩ | ⟨it', hs, h⟩ | ⟨hd, h⟩ := successor_matchStep h
+  · cases successor_yield.mp h
+    apply FlatMap.lex_of_right
     exact Or.inl ⟨_, hy⟩
-  · cases up_successor_skip.mp h
-    apply Flatten.lex_of_right
+  · cases successor_skip.mp h
+    apply FlatMap.lex_of_right
     exact Or.inr hs
-  · apply Flatten.lex_of_left
+  · apply FlatMap.lex_of_left
     exact descending_flattenStepNone h
 
 -- TODO: put this into core
@@ -178,106 +175,63 @@ theorem Option.wellFounded_lt {α} {rel : α → α → Prop} (h : WellFounded r
     · exact hn
     · exact ih _ hyx'
 
-instance [Monad m] [Iterator α m α'] [Iterator α' m β] [Finite α m] [Finite α' m] :
-    Finite (Flatten α α') m := by
-  refine finite_instIterator (m := m) _ (rel := rel m) ?_ ?_
-  · simp only [rel, Flatten.lex]
+instance [Monad m] [Iterator α α' m β] [Iterator α₂ α₂' m γ] [Finite α m] [Finite α₂ m] :
+    SimpleIterator.Finite (FlatMap α f) m where
+  rel := rel m f
+  wf := by
+    simp only [rel, FlatMap.lex]
     apply InvImage.wf
     refine ⟨fun (a, b) => Prod.lexAccessible (WellFounded.apply ?_ a) (WellFounded.apply ?_) b⟩
     · exact InvImage.wf _ Finite.wf
     · exact Option.wellFounded_lt <| InvImage.wf _ Finite.wf
-  · intro it it' h
+  subrelation {it it'} h := by
+    simp only [SimpleIterator.step] at h
     split at h
-    · apply Flatten.lex_of_left
+    · apply FlatMap.lex_of_left
       exact descending_flattenStepNone h
     · exact descending_flattenStepSome h
 
 end Finite
 
-section General
-
-section FlatMapH
-
-variable {α : Type u} {β : Type v} {m : Type w → Type w'} [Monad m]
-  {α' : Type u'} {β' : Type v'} {f : (b : β) → α'}
-
-/--
-Given an iterator `it`, a heterogeneous iterator-valued mapping function `f`
-and monad transformations `fm` and `fn`, `it.flatMapH f mf` is an iterator that applies
-`f` to each output of `it` to obtain an inner iterator.
-The `flatMap` iterator will yield all of the outputs of such an inner iterator before making the
-next step with `it`. In other words, `it` flattens the iterator of iterators obtained by mapping with `f`.
-
-**Marble diagram:**
-
-```text
-it                 ---a    ---b     c    --d--⊥
-f a                   a1-a2⊥
-f b                           b1-b2 ⊥
-f c                                 c1-c2⊥
-f d                                        ⊥
-it.flatMapH        ---a1-a2---b1-b2 c1-c2  ---⊥
-```
-
-Note that it is always possible for the implementation to insert some skip steps in between.
-The insertion of additional skip steps is an implementation detail and should not be relevant
-for any consumer.
-
-**Termination properties:**
-
-* `Finite` instance: only if `it` and all of the iternal iterators are finite
-* `Productive` instance: only if `it` it finite and all of the internal iterators are productive
-
-_TODO:_ implement the `Productive` instance
-
-**Performance:**
-
-This combinator incurs an additional O(1) cost with each output of `it` or an internal stream.
-
-_TODO_: Improve this so that the cost is only incurred with each output of `it`. This should at
-least work for internal iterator types that contain a computationally cheap empty iterator.
--/
-@[inline]
-def Iter.flatMapH (f : β → α') [Iterator α m β] (it : Iter (α := α) m β) [Iterator α' m β'] [Monad m] :=
-  (it.mapH f |>.flatten : Iter m β')
-
-end FlatMapH
-
 section Dependent
 
-universe v u
+variable {m : Type w → Type w'}
+  {β : Type w} {α : β → Type w} {α' : β → Type u'} {γ : Type v}
 
-structure SigmaIterator (β : Type u) (α : β → Type u') where
+structure SigmaIterator {β : Type v} (α : β → Type w) where
   b : β
   inner : α b
 
-def SigmaIterator.lex {β : Type u} {α : β → Type u'} (r : (b : β) → α b → α b → Prop) :
-    SigmaIterator β α → SigmaIterator β α → Prop :=
+def SigmaIterator.lex (r : (b : β) → α b → α b → Prop) :
+    SigmaIterator α → SigmaIterator α → Prop :=
   InvImage (PSigma.Lex emptyRelation r) (fun it => ⟨it.b, it.inner⟩)
 
-theorem SigmaIterator.lex_of_right {β : Type u} {α : β → Type u'} (r : (b : β) → α b → α b → Prop)
+theorem SigmaIterator.lex_of_right (r : (b : β) → α b → α b → Prop)
     {b it it'} (h : r b it it') : SigmaIterator.lex r ⟨b, it⟩ ⟨b, it'⟩ :=
   PSigma.Lex.right _ h
 
-def SigmaIterator.rel (m : Type w → Type w') {β : Type u} {α : β → Type u'} [∀ b, Iterator (α b) m β'] :
-    SigmaIterator β α → SigmaIterator β α → Prop :=
+variable (m) in
+def SigmaIterator.rel [∀ b, Iterator (α b) (α' b) m γ] :
+    SigmaIterator α → SigmaIterator α → Prop :=
   SigmaIterator.lex (fun _ => InvImage FiniteIteratorWF.lt (finiteIteratorWF (m := m)))
 
-instance {β : Type v} {α : β → Type u'} {γ : Type v'}
-    {m : Type w → Type w'} [Monad m] [∀ b, Iterator (α b) m γ] :
-    Iterator (SigmaIterator β α) m γ :=
-  Iteration.instIterator fun it => do
-    matchStep it.inner
-      (fun it' c => pure <| .yield ⟨it.b, it'⟩ c ⟨⟩)
+instance {β : Type w} {α : β → Type w} {α' : β → Type u'}
+    [Monad m] [∀ b, Iterator (α b) (α' b) m γ] :
+    SimpleIterator (SigmaIterator α) (SigmaIterator α') m γ where
+  βInternal := (b : β) × Iterator.βInternal (α := α b) (m := m)
+  αEquiv := sorry
+  βEquiv := sorry
+  step it := by
+    exact matchStep it.inner
+      (fun it' c => pure <| .yield ⟨it.b, it'⟩ ⟨it.b, Iterator.βEquiv.hom c⟩ ⟨⟩)
       (fun it' => pure <| .skip ⟨it.b, it'⟩ ⟨⟩)
       (pure <| .done ⟨⟩)
 
-instance {β : Type u} {α : β → Type max u v} {γ : Type w}
-    {m : Type w → Type w'} [Monad m]
-    [∀ b, Iterator (α b) m γ] [∀ b, Finite (α b) m] : Finite (SigmaIterator β α) m := by
-  refine finite_instIterator _ (rel := ?_) ?_ ?_
-  · exact SigmaIterator.rel m
-  · rw [SigmaIterator.rel]
+instance {β : Type w} {α : β → Type w} {α' : β → Type u'}
+    [Monad m] [∀ b, Iterator (α b) (α' b) m γ] [∀ b, Finite (α b) m] : SimpleIterator.Finite (SigmaIterator α) m where
+  rel := SigmaIterator.rel m
+  wf := by
+    rw [SigmaIterator.rel]
     apply InvImage.wf
     refine ⟨fun ⟨b, it⟩ => ?_⟩
     apply PSigma.lexAccessible
@@ -285,25 +239,28 @@ instance {β : Type u} {α : β → Type max u v} {γ : Type w}
     · intro a
       apply InvImage.wf
       exact Finite.wf
-  · intro it it' h
-    obtain ⟨_, _, hy, h⟩ | ⟨_, hs, h⟩ | ⟨hd, h⟩ := prop_successor_matchStep h
-    · cases up_successor_yield.mp h
+  subrelation {it it'} h := by
+    obtain ⟨_, _, hy, h⟩ | ⟨_, hs, h⟩ | ⟨hd, h⟩ := successor_matchStep h
+    · cases successor_yield.mp h
       apply SigmaIterator.lex_of_right
       exact Or.inl ⟨_, hy⟩
-    · cases up_successor_skip.mp h
+    · cases successor_skip.mp h
       apply SigmaIterator.lex_of_right
       exact Or.inr hs
-    · cases up_successor_done.mp h
+    · cases successor_done.mp h
 
 variable {α : Type u} {β : Type v} {m : Type w → Type w'} [Monad m]
   {α' : β → Type u'} {β' : Type v'} {f : (b : β) → α' b}
 
+end Dependent
+
+section Iter
 /--
-Given an iterator `it`, a dependently typed, heterogeneous iterator-valued mapping function `f`
-and monad transformations `fm` and `fn`, `it.flatMapHD f mf` is an iterator that applies
-`f` to each output of `it` to obtain an inner iterator.
-The `flatMap` iterator will yield all of the outputs of such an inner iterator before making the
-next step with `it`. In other words, `it` flattens the iterator of iterators obtained by mapping with `f`.
+Given an iterator `it` and an iterator-valued mapping function `f`,
+`it.flatMap f` is an iterator that applies `f` to each output of `it` and concatenates all of the iterators
+obtained by applying `f`.
+It will yield all of the outputs of the current inner inner iterator before making the
+next step with `it`.
 
 **Marble diagram:**
 
@@ -313,7 +270,7 @@ f a                   a1-a2⊥
 f b                           b1-b2 ⊥
 f c                                 c1-c2⊥
 f d                                        ⊥
-it.flatMapHD       ---a1-a2---b1-b2 c1-c2  ---⊥
+it.flatMap         ---a1-a2---b1-b2 c1-c2  ---⊥
 ```
 
 Note that it is always possible for the implementation to insert some skip steps in between.
@@ -334,12 +291,71 @@ This combinator incurs an additional O(1) cost with each output of `it` or an in
 _TODO_: Improve this so that the cost is only incurred with each output of `it`. This should at
 least work for internal iterator types that contain a computationally cheap empty iterator.
 -/
-@[inline]
-def Iter.flatMapHD (f : (b : β) → α' b) [Iterator α m β] (it : Iter (α := α) m β)
-    [∀ b, Iterator (α' b) m β'] [Monad m] :=
-  (it.mapH (fun b => SigmaIterator.mk b (f b)) |>.flatten : Iter m β')
+@[always_inline, inline]
+def Iter.flatMap {α : Type w} {α' : Type u} {β : Type v} {α₂ : Type w} {α₂' : Type u₂}
+    {γ : Type x} {m : Type w → Type w'}
+    [Monad m] [Iterator α α' m β] [Iterator α₂ α₂' m γ] (f : β → Iter (α := α₂) m γ)
+    (it : Iter (α := α) m β) :=
+  (toIter m <| FlatMap.init it.inner (Iter.inner ∘ f) : Iter m γ)
 
-end Dependent
+@[always_inline, inline]
+def Iter.flatMapS {α : Type w} {α' : Type w} {β : Type v} {α₂ : Type w} {α₂' : Type w}
+    {γ : Type x} {m : Type w → Type w'}
+    [Monad m] [Iterator α α' m β] [Iterator α₂ α₂' m γ] (f : β → Iter (α := α₂) m γ)
+    (it : Iter (α := α) m β) :=
+  (toIter m <| FlatMap.init it.inner (Iter.inner ∘ f) : Iter m γ)
+
+/--
+Given an iterator `it` and a dependently typed, iterator-valued mapping function `f`, `it.flatMapD f`
+is an iterator that applies `f` to each output of `it` and concatenates all of the iterators
+obtained by applying `f`.
+It will yield all of the outputs of the current inner inner iterator before making the
+next step with `it`.
+
+**Marble diagram:**
+
+```text
+it                 ---a    ---b     c    --d--⊥
+f a                   a1-a2⊥
+f b                           b1-b2 ⊥
+f c                                 c1-c2⊥
+f d                                        ⊥
+it.flatMapD        ---a1-a2---b1-b2 c1-c2  ---⊥
+```
+
+Note that it is always possible for the implementation to insert some skip steps in between.
+The insertion of additional skip steps is an implementation detail and should not be relevant
+for any consumer.
+
+**Termination properties:**
+
+* `Finite` instance: only if `it` and all of the iternal iterators are finite
+* `Productive` instance: only if `it` it finite and all of the internal iterators are productive
+
+_TODO:_ implement the `Productive` instance
+
+**Performance:**
+
+This combinator incurs an additional O(1) cost with each output of `it` or an internal stream.
+
+_TODO_: Improve this so that the cost is only incurred with each output of `it`. This should at
+least work for internal iterator types that contain a computationally cheap empty iterator.
+-/
+@[always_inline, inline]
+def Iter.flatMapD {α : Type w} {α' : Type u} {β : Type v} {α₂ : β → Type w} {α₂' : β → Type u₂}
+    {γ : Type x} {m : Type w → Type w'} [Monad m] [Iterator α α' m β] [∀ b, Iterator (α₂ b) (α₂' b) m γ]
+    (f : (b : β) → Iter (α := α₂ b) m γ) (it : Iter (α := α) m β) :=
+  let βEquiv := Iterator.βEquiv (α := α) (m := m)
+  -- TODO: why does this cause an error if I use `let`?
+  letI σit b := toIter m <| SigmaIterator.mk (α := (α₂ <| βEquiv.inv ·)) (βEquiv.hom b)
+    (by
+      simp only [βEquiv.inv_hom]
+      exact (f b).inner)
+  (it.flatMap σit : Iter m γ)
+
+end Iter
+
+#exit
 
 section Simple
 
