Iterator/MWE.lean
@@ -1,10 +1,38 @@
 import Iterator.Generators
 import Iterator.Combinators.Take
+import Iterator.Combinators.FilterMap
+import Iterator.Combinators.FlatMap
 
 set_option trace.compiler.ir.result true in
 set_option compiler.small 2 in
 def test (l : List Nat) : Nat :=
-  go (l.iter Id |>.take 5) 0
+  go (l.iter Id |>.map (· * 2) |>.take 5) 0
+where
+  go it acc :=
+    match it.step with
+    | .yield it' x _ => go it' (acc + x)
+    | .skip it' _ => go it' acc
+    | .done _ => acc
+  termination_by it.terminationByFinite
+
+set_option pp.universes true in
+set_option pp.explicit true in
+def firstOfEach {α} (l : List (List α)) :=
+  let it := List.iter l Id |>.flatMapS (List.iter · Id)
+  go (it) 0
+where
+  go it acc : Nat :=
+    match it.step with
+    | .yield it' x _ => sorry --go it' acc --(acc + x)
+    | .skip it' _ => sorry--go it' acc
+    | .done _ => acc
+  termination_by it-- .terminationByFinite
+  decreasing_by all_goals sorry
+
+set_option trace.compiler.ir.result true in
+set_option compiler.small 2 in
+def test2 (l : List Nat) : Nat :=
+  go (l.iter Id |>.map (· * 2) |>.take 5) 0
 where
   go it acc :=
     match it.step with
